src/coq/CFG.v
@@ -9,77 +9,77 @@
  ---------------------------------------------------------------------------- *)
 
 Require Import ZArith List String Omega.
-Require Import Vellvm.AstLib Vellvm.Ollvm_ast.
+Require Import Vellvm.AstLib Vellvm.Ollvm_ast Vellvm.Dom.
 Require Import Vellvm.Classes.
 Import ListNotations.
 
-(* paths into a program ----------------------------------------------------- *)
+Definition pt := instr_id.
 
-Record path :=
-  mk_path {
+(* program counter is a function plus instruction id ------------------------ *)
+
+Record pc :=
+  mk_pc {
       fn  : function_id;
-      bn  : block_id;
-      ins : instr_id;
+      ins : pt;
     }.
 
-Definition string_of_path p : string :=
-  "@" ++ (string_of_raw_id (fn p)) ++ ":" ++ (string_of_raw_id (bn p)) ++ ":" ++ (string_of_instr_id (ins p)).
+Definition string_of_pc p : string :=
+  "@" ++ (string_of_raw_id (fn p)) ++ (* ":" ++ (string_of_raw_id (bn p)) ++ *) ":" ++ (string_of_instr_id (ins p)).
 
 
 Require Import Equalities.
-Module PATH <: UsualDecidableTypeFull.
-  Definition t := path.
+Module PC <: UsualDecidableTypeFull.
+  Definition t := pc.
   Include HasUsualEq.
   Include UsualIsEq.
   Include UsualIsEqOrig.
   
-  Lemma eq_dec : forall (x y : path), {x = y} + {x <> y}.
+  Lemma eq_dec : forall (x y : pc), {x = y} + {x <> y}.
   Proof.
     intros x y.
-    destruct x as [xf xb xi]; destruct y as [yf yb yi].
+    destruct x as [xf xi]; destruct y as [yf yi].
     destruct (xf == yf).
-    - destruct (xb == yb).
       + destruct (xi == yi).
         * subst. left. reflexivity.
         * right. unfold not. intros. apply n. inversion H. auto.
       + right. unfold not. intros. apply n. inversion H. auto.
-    - right. unfold not. intros. apply n. inversion H. auto.
   Qed.
 
   Include HasEqDec2Bool.
   
-End PATH.
-Instance eq_dec_path : eq_dec path := PATH.eq_dec.
+End PC.
+Instance eq_dec_pc : eq_dec pc := PC.eq_dec.
 
 
 (* control flow graphs (CFGs) ----------------------------------------------- *)
 
-(* The path p in the step is the "fallthrough" to the next instruction. *)
 Inductive cmd : Set :=
-| Step  (i:instr) (p:path)
-| Jump  (t:terminator)
+| Step  (i:instr) (next:pt)
+| Jump  (bn:block_id) (t:terminator)
 .                    
 
 Inductive block_entry : Set :=
-| Phis (phis : list (local_id * instr)) (p:path)
+| Phis (phis : list (local_id * instr)) (next:pt)
 .
 
+(* each function definition corresponds to a control-flow graph *)
 Record cfg := mkCFG
 {
-  init : path;
-  code : path  -> option cmd; 
-  funs : function_id -> option (list ident * block_id * instr_id);  
-  blks : function_id -> block_id -> option block_entry;  
+  init : pt;
+  code : pt -> option cmd; 
+  blks : block_id -> option instr_id;
+  phis : block_id -> option block_entry;
 }.
 
+
 (* structurally well-formed CFGs 
-   - the initial path denotes a command  
-   - fallthrough closure: each fallthrough path maps to a command 
+   - the initial pt denotes a command  
+   - fallthrough closure: each fallthrough pt maps to a command 
    - jump closure: each label used in a terminator leads to a
      block within the same function body.
 *)
 
-Definition path_exists (CFG : cfg) (p:path) : Prop :=
+Definition pt_exists (CFG : cfg) (p:pt) : Prop :=
   exists cmd, (code CFG p) = Some cmd.
 
 Definition lbls (t:terminator) : list block_id :=
@@ -94,118 +94,260 @@ Definition lbls (t:terminator) : list block_id :=
   | TERM_Invoke  _ _ l1 l2 => [l1; l2] 
   end.
 
+Definition is_phi (i:instr) : Prop :=
+  match i with
+   | INSTR_Phi _ _ => True
+   | _ => False
+  end.
 
+
+(** Edge relation *)
+Inductive succ_pt (g:cfg) : pt -> pt -> Prop :=
+| succ_pt_S : forall p i q,
+    (code g) p = Some (Step i q) ->
+    succ_pt g p q
+| succ_pt_J : forall p b t l q,
+    (code g) p = Some (Jump b t) ->
+    In l (lbls t) ->
+    (blks g) l = Some q ->
+    succ_pt g p q.
+
+(*
+    (blks g) (fn p) l = Some (Phis ((x,ins)::tl) q) ->
+    succ_pt g p (mk_pt (fn p) (IId x))
+| succ_pt_Jnophi: forall p b t l q,
+    (code g) p = Some (Jump b t) ->
+    In l (lbls t) ->
+    (blks g) (fn p) l = Some (Phis [] q) ->
+    succ_pt g p q.
+*)
+
+Inductive wf_phis (CFG : cfg) (q : pt) : pt -> list (local_id * instr) -> Prop :=
+| wf_phis_nil : wf_phis CFG q q []
+| wf_phis_cons :
+    forall p p' x t args rest,
+    (code CFG p) = Some (Step (INSTR_Phi t args) p') ->
+    wf_phis CFG q p' rest ->
+    wf_phis CFG q p ((x, INSTR_Phi t args) :: rest) .
+            
 Definition wf_cfg (CFG : cfg) : Prop :=
-  path_exists CFG (init CFG) 
-  /\ (forall fn args bn ins, (funs CFG fn) = Some (args, bn, ins) -> path_exists CFG (mk_path fn bn ins)) 
-  /\ (forall p q i, (code CFG p) = Some (Step i q) -> path_exists CFG q)
-  /\ (forall p t, (code CFG p) = Some (Jump t) ->
-    Forall (fun bn => exists phis, exists q, (blks CFG (fn p) bn) = Some (Phis phis q) /\ path_exists CFG q) (lbls t)).
+  pt_exists CFG (init CFG) 
+  /\ (forall p q i, (code CFG p) = Some (Step i q) -> pt_exists CFG q)
+  /\ (forall p bn t, (code CFG p) = Some (Jump bn t) ->
+               Forall (fun bn => exists p', exists xs, exists q,
+                             (blks CFG bn) = Some p' 
+                             /\ (phis CFG bn) = Some (Phis xs q) 
+                             /\ wf_phis CFG q p' xs
+                             /\ pt_exists CFG q
+                      )
+                      (lbls t)).
 
-
-
-
-
-
-
-
+Lemma wf_cfg_succ_pt : forall g p1 p2, wf_cfg g -> pt_exists g p1 -> succ_pt g p1 p2 -> pt_exists g p2.
+Proof.
+  intros g p1 p2 H H0 H1.
+  destruct H as [Hinit [HStep HJump]].
+  inversion H1; subst.
+  - eapply HStep. apply H.
+  - apply HJump in H.
+    eapply Forall_forall in H.
+    Focus 2. apply H2.
+    destruct H as [p' [xs [q [Ha [Hb [Hc Hd]]]]]].
+    rewrite H3 in Ha. inversion Ha. subst.
+    induction Hc.
+    * exact Hd.
+    * exists (Step (INSTR_Phi t0 args) p').
+      exact H.
+Qed.      
 
 
 
 (* creating CFGs from syntax ------------------------------------------------ *)
-
-Fixpoint entities_to_init ets : option path :=
+         
+Fixpoint lookup_function_definition ets f : option definition :=
   match ets with
-    | [] => None
-    | (TLE_Definition d) :: t =>
-      if (dc_name (df_prototype d)) == (Name "main") then
-        match (df_instrs d) with
-          | [] => None
-          | b :: _ => Some (match blk_instrs b with
-                        | [] => mk_path (Name "main") (blk_id b) (blk_term_id b)
-                        | (iid, _) :: t => mk_path (Name "main") (blk_id b) iid
-                            end)
-        end
-      else entities_to_init t
-    | _ :: t => entities_to_init t
+  | [] => None
+  | (TLE_Definition d) :: ts =>
+    if (dc_name (df_prototype d)) == f then
+      Some d
+    else
+      lookup_function_definition ts f
+  | _ :: ts => lookup_function_definition ts f
+  end.
+                                                 
+Fixpoint init_of_definition d : option pt :=
+  match (df_instrs d) with
+  | [] => None
+  | b :: _ => Some (match blk_instrs b with
+                   | [] => blk_term_id b
+                   | (iid, _) :: t => iid
+                   end)
   end.
 
-Fixpoint entities_to_funs ets fid :=
-  match ets with
-    | [] => None
-    | (TLE_Definition d) :: t =>
-      if (dc_name (df_prototype d)) == fid then
-        match df_instrs d with
-          | [] => None
-          | b :: _ => Some (match blk_instrs b with
-                              | [] => (map (fun x => ID_Local x) (df_args d), blk_id b, blk_term_id b)
-                              | (iid, _) :: t => (map (fun x => ID_Local x) (df_args d), blk_id b, iid)
-                            end)
-        end
-      else entities_to_funs t fid
-    | _ :: t => entities_to_funs t fid
-  end.
 
-Fixpoint phis_from_block fname bname term_id (b : list (instr_id * instr)) : option block_entry :=
+Fixpoint phis_from_block term_id (b : list (instr_id * instr)) : option block_entry :=
   match b with
     | (IId iid, INSTR_Phi i v as ins) :: t =>
-       'rest <- phis_from_block fname bname term_id t;
+       'rest <- phis_from_block term_id t;
         match rest with
           | Phis phis p => Some (Phis ((iid, ins)::phis) p) 
         end
     | (IVoid _, INSTR_Phi i v as ins) :: t => None
-    | (next, _) :: _ => Some (Phis [] {| fn := fname; bn := bname; ins := next |})
-    | [] => Some (Phis [] {| fn := fname; bn := bname; ins := term_id |})
+    | (next, _) :: _ => Some (Phis [] next)
+    | [] => Some (Phis [] term_id)
   end.
 
-Fixpoint entities_to_blks ets fid bid : option block_entry :=
-  match ets with
-    | [] => None
-    | (TLE_Definition d) :: t =>
-      if (dc_name (df_prototype d)) == fid then
-        'bs <- find (fun b => RawID.eqb bid (blk_id b)) (df_instrs d);
-        phis_from_block fid bid (blk_term_id bs) (blk_instrs bs) 
-      else entities_to_blks t fid bid
-    | _ :: t => entities_to_blks t fid bid
-  end.
+Fixpoint lookup_block bs block_id : option block :=
+  find (fun b => if (blk_id b) == block_id then true else false) bs.
 
-Definition next_or_term term_id (is : list (instr_id * instr)) : instr_id :=
+Fixpoint block_to_phis (b:block) : option block_entry :=
+  phis_from_block (blk_term_id b) (blk_instrs b).
+  
+Definition fallthrough term_id (is : list (instr_id * instr)) : instr_id :=
   match is with
   | [] => term_id
   | (next, _)::_ => next
   end.
 
-Fixpoint cmd_from_block to_find fn bn term_id is : option cmd :=
-  match is with
-    | [] => None
-    | (id, ins) :: rest =>
-      if to_find == id then
-        Some (Step ins (mk_path fn bn (next_or_term term_id rest)))
-      else cmd_from_block to_find fn bn term_id rest
+Fixpoint lookup_instr (p:pt) term_id (insns : list (instr_id * instr)) : option cmd :=
+  match insns with
+  | [] =>  None
+  | (x,ins)::rest =>
+    if p == x then
+      Some (Step ins (fallthrough term_id rest))
+    else
+      lookup_instr p term_id rest
   end.
 
-Fixpoint cmd_from_term to_find (term_id:instr_id) term : option cmd :=
-  if to_find == term_id then Some (Jump term) else None.
+Definition cmd_from_block (p:pt) (b:block) : option cmd :=
+  if (blk_term_id b == p) then
+    Some (Jump (blk_id b) (blk_term b))
+  else
+    lookup_instr p (blk_term_id b) (blk_instrs b).
 
-Fixpoint entities_to_code ets (p : path) : option cmd :=
-  match ets with
-    | [] => None
-    | (TLE_Definition d) :: t =>
-      if (dc_name (df_prototype d)) == (fn p) then
-        'b <- find (fun b => RawID.eqb (bn p) (blk_id b)) (df_instrs d);
-        match cmd_from_block (ins p) (fn p) (bn p) (blk_term_id b) (blk_instrs b) with
-          | Some x => Some x
-          | None => cmd_from_term (ins p) (blk_term_id b) (blk_term b)
-        end
-      else entities_to_code t p
-    | _::t => entities_to_code t p
+
+Fixpoint cmd_from_blocks (p:pt) (bs:list block) : option cmd := 
+match bs with
+  | [] => None
+  | b :: bs =>
+    match cmd_from_block p b with
+    | None => cmd_from_blocks p bs
+    | Some cmd => Some cmd
+    end
   end.
 
-Definition TLE_to_cfg tl :=
-  'init <- entities_to_init tl;
-  Some {| init := init;
-          code := entities_to_code tl;
-          blks := entities_to_blks tl;
-          funs := entities_to_funs tl
-       |}.
+Definition code_of_definition (d:definition) (p:pt) : option cmd :=
+  cmd_from_blocks p (df_instrs d).
+  
 
+Definition blks_of_definition (d:definition) block_id : option pt :=
+  'b <- lookup_block (df_instrs d) block_id;
+  Some (fallthrough (blk_term_id b) (blk_instrs b)).
+
+Definition phis_of_definition (d:definition) block_id : option block_entry :=
+  'b <- lookup_block (df_instrs d) block_id;
+  block_to_phis b.
+
+Definition cfg_of_definition (d:definition) : option cfg :=
+  'init <- init_of_definition d;
+    Some {| init := init;
+            code := code_of_definition d;
+            blks := blks_of_definition d;
+            phis := phis_of_definition d
+         |}.
+            
+Definition fcfg := function_id -> option (list ident * cfg).
+
+Fixpoint entities_to_funs ets fid : option (list ident * cfg) :=
+  'd <- lookup_function_definition ets fid;
+  'cfg <- cfg_of_definition d;
+  Some (map (fun x => ID_Local x) (df_args d), cfg).
+
+
+(*
+
+Module Wellformedness.
+
+
+  (** *** GRAPH instance for dominance calculation *)
+
+
+  (** Graph of program points *)
+
+  Module PcGraph <: GRAPH.
+    Definition t := cfg.
+    Definition V := pt.
+    Definition entry g := init g.
+    Definition Succ := succ_pt.
+    Definition Mem := pt_exists.
+  End PcGraph.
+
+  Module Export Dom := Dom.Spec PcGraph.
+
+  (** *** Definitions for Well-formed SSA programs. *)
+
+  (** FULL: Most of the Vminus instructions define the uid associated
+  with their program point.  Some (like [store] and the [tmn]s)
+  do not. *)
+  (** TERSE: The command at the given [pc] defines uid. *)
+
+  Definition def_at_pc (g:cfg) (p:pt) (uid:uid) : Prop :=
+    exists c, insn_at_pc g p (uid, c) /\ defs_uid (uid, c). 
+
+  (** The definition of [uid] strictly dominates the pc. *)
+ 
+  Definition uid_sdom_pc (g:Cfg.t) (uid:uid) (p:pc) : Prop :=
+    exists p', def_at_pc g p' uid /\ SDom g p' p.
+
+  (** All uses of a [uid] must be strictly dominated by
+      their definitions. *)
+
+  Definition wf_use (g:Cfg.t) (i:insn) (p:pc) : Prop :=
+    forall uid, In (val_uid uid) (insn_uses i) -> uid_sdom_pc g uid p.
+
+  (** All jump targets must be legal block labels. *)
+
+  Definition wf_lbl (g:Cfg.t) (i:insn) : Prop :=
+    forall l, In l (insn_lbls i) -> wf_pc g (block_entry l).
+
+  (** *** Well-formed phi nodes *)
+
+  (**  Consider [ %x = phi [lbl1:v1, ...,lbln:vn] ].  This is well formed
+       when every predecessor block with terminator program point p' 
+       has a label associated with value v.  Moreover, if v is a uid then
+       the definition of the uid strictly dominates p'.
+  *)
+
+  Definition wf_phi_args (g:Cfg.t) (i:insn) (p:pc) : Prop :=
+    forall pred, succ_pt g pred (entry_of_pc p) ->
+      (exists v, In (lbl_of pred, v) (insn_phis i)) /\
+      (forall uid, In (lbl_of pred, val_uid uid) (insn_phis i) -> 
+          uid_sdom_pc g uid pred).
+
+  Definition wf_phi_pred (g:Cfg.t) (i:insn) (p:pc) : Prop :=
+    forall l v, In (l, v) (insn_phis i) ->
+      (exists pred, succ_pt g pred (entry_of_pc p) /\ lbl_of pred = l).
+
+  Definition wf_phi (g:Cfg.t) (i:insn) (p:pc) : Prop :=
+    is_phi i -> wf_phi_args g i p
+             /\ wf_phi_pred g i p
+             /\ insn_phis i <> [].
+
+  (** *** Well-formed instructions *)
+
+  Inductive wf_insn (g:Cfg.t) : insn -> pc -> Prop :=
+  | wf_insn_intro : forall i p,
+      wf_use g i p ->
+      wf_lbl g i ->
+      wf_phi g i p ->
+      wf_insn g i p.
+
+  Inductive wf_prog (g:Cfg.t) : Prop :=
+  | wf_prog_intro : forall
+      (Hwfcfg : wf_cfg g)
+      (Hwfis : forall p i, insn_at_pc g p i -> wf_insn g i p)
+      (Hwftmn : forall p' i, tmn_pc g p' -> insn_at_pc g p' i -> is_tmn i)
+      (Hwfentry : forall p, ~ succ_pt g p (block_entry (entry_block g))),
+      wf_prog g.
+
+End Wellformedness.
+*)
