src/coq/Dom.v
@@ -1,0 +1,250 @@
+
+
+(** Reasoning about dominators in a graph. *)
+
+Require Import List Equalities Orders RelationClasses.
+Require Import FSets FMaps.
+Import ListNotations.
+Require Import Vellvm.Util.
+
+
+Module Type LATTICE.
+  Include EqLe'.
+
+  Declare Instance eq_equiv : Equivalence eq.
+  Declare Instance le_preorder : PreOrder le.
+  Declare Instance le_poset : PartialOrder eq le.
+  
+  Parameter eq_dec : forall x y, {x == y} + {x ~= y}.
+
+  Parameter bot : t.
+  Axiom le_bot : forall x, bot <= x.
+
+  Parameter top : t.
+  Axiom le_top : forall x, x <= top.
+
+  Parameter join : t -> t -> t.
+  Axiom le_join_l : forall x y, x <= join x y.
+  Axiom le_join_r : forall x y, y <= join x y.
+End LATTICE.
+
+Module BoundedSet(Import S:FSetInterface.WS) <: LATTICE.
+
+  Module Import SFacts := FSetFacts.WFacts S.
+
+  Definition t : Type := option S.t.
+
+  Definition eq (t1 t2: t) : Prop :=
+    match t1, t2 with
+      | Some s1, Some s2 => s1 [=] s2
+      | None, None => True
+      | _, _ => False
+    end.
+
+  Definition le (t1 t2: t) : Prop :=
+    match t1, t2 with
+      | Some s1, Some s2 => s2 [<=] s1
+      | None, Some _ | None, None => True
+      | Some _, None => False
+    end.
+
+  Include EqLeNotation.
+
+  Instance eq_equiv : Equivalence eq.
+  Proof.
+    constructor.
+    red. destruct x; simpl; intuition.
+    red. destruct x, y; simpl; intros; intuition.
+    red. destruct x, y, z; simpl; intros; intuition.
+    transitivity t1; auto.
+  Qed.
+
+  Instance le_preorder : PreOrder le.
+  Proof.
+    constructor.
+    red. destruct x; simpl; intuition. 
+    red. destruct x, y, z; simpl; intros; intuition.
+    transitivity t1; auto.
+  Qed.
+
+  Instance le_poset : PartialOrder eq le.
+  Proof.
+    constructor.
+    intro. repeat red. split.
+    destruct x, x0; simpl in *; intuition. 
+    unfold Subset. intros. rewrite H; auto.
+    red. destruct x, x0; simpl in *; intuition.
+    unfold Subset. intros. rewrite <- H. auto.
+
+    destruct x, x0; simpl; 
+      intros H; repeat red in H; simpl in H; 
+      intuition.
+    repeat red in H1. repeat red in H0.
+    red; intuition.
+  Qed.
+
+  Definition eq_dec : forall x y, {x == y} + {x ~= y}.
+    refine (fun t1 t2 => match t1, t2 with
+                           | Some s1, Some s2 => _
+                           | None, None => left _
+                           | _, _ => right _
+                         end); auto using S.eq_dec.
+  Defined.
+
+  Definition bot : t := None.
+
+  Lemma le_bot : forall x, bot <= x.
+  Proof.
+    simpl; destruct x; trivial.
+  Qed.
+
+  Definition top : t := Some S.empty.
+  Lemma le_top : forall x, x <= top.
+  Proof. 
+    simpl. destruct x; trivial. red. intros.
+    exfalso. eapply empty_iff; eauto. 
+  Qed.
+
+  Definition join (t1 t2: t) : t :=
+    match t1, t2 with
+      | Some s1, Some s2 => Some (S.inter s1 s2) 
+      | None, Some s | Some s, None => Some s
+      | None, None => None
+    end.
+
+  Lemma le_join_l : forall x y, x <= join x y.
+  Proof.
+    intros. destruct x, y; repeat red; auto.
+    intros. eapply inter_1; eauto.
+  Qed.
+
+  Lemma le_join_r : forall x y, y <= join x y.
+  Proof.
+    intros. destruct x, y; repeat red; auto.
+    intros. eapply inter_2; eauto.
+  Qed.
+
+  Definition union (t1 t2: t) : t :=
+    match t1, t2 with
+      | Some s1, Some s2 => Some (S.union s1 s2) 
+      | None, Some s | Some s, None => None
+      | None, None => None
+    end.
+    
+  Definition singleton (e:S.elt) : t := Some (S.singleton e).
+
+  Definition In (e:S.elt) (t:t) : Prop :=
+    match t with
+      | Some s => S.In e s
+      | None => True
+    end.
+
+End BoundedSet.
+
+
+
+(** ** GRAPH *)
+(** Interface for a nonempty graph [t] with: 
+     - a set of _vertices_ of type [V]
+     - a distinguished _entry vertex_
+     - an _edge relation_ [Succ]
+*)
+
+Module Type GRAPH.
+  Parameter Inline t V : Type.
+  
+  Parameter Inline entry : t -> V.
+  Parameter Inline Succ : t -> V -> V -> Prop.
+  Parameter Inline Mem : t -> V -> Prop.
+End GRAPH.
+
+(** ** Specification of Dominators *)
+
+Module Spec (Import G:GRAPH).
+
+(** Defines a path in the graph. *)
+
+  Inductive Path (g:G.t) : V -> V -> list V -> Prop :=
+  | path_nil : forall v, 
+      Mem g v -> Path g v v [v]
+  | path_cons : forall v1 v2 v3 vs,
+      Path g v1 v2 vs -> Mem g v3 -> Succ g v2 v3 
+      -> Path g v1 v3 (v3::vs).
+
+(** *** Definition of domination *)
+
+  Definition Dom (g:G.t) (v1 v2: V) : Prop :=
+    forall vs, Path g (entry g) v2 vs -> In v1 vs.
+
+  Definition SDom (g:G.t) (v1 v2 : V) : Prop :=
+    v1 <> v2 /\ Dom g v1 v2.
+
+  Lemma dom_step : forall g v1 v2,
+    Mem g v2 -> Succ g v1 v2 -> forall v', SDom g v' v2 -> Dom g v' v1.
+(* FOLD *)
+  Proof.
+    unfold SDom, Dom. intros g v1 v2 Hmem Hsucc v' [Hneq Hdom] p Hp.
+    cut (In v' (v2::p)). inversion 1; subst; intuition. 
+    apply Hdom. eapply path_cons; eauto. 
+  Qed.
+(* /FOLD *)
+
+End Spec.
+
+(** *** Relate an algorithm to the specification *)
+Module Type Algdom (Import G:GRAPH).
+  Module Import GS := Spec G.
+
+  Declare Module E : UsualDecidableType with Definition t := V.
+  Declare Module NS : FSetInterface.WS with Module E:=E.
+  Module L := BoundedSet NS.
+  Include EqLeNotation L.
+
+  Parameter calc_sdom : G.t -> option (V -> L.t).
+
+  Axiom entry_sound : forall g sdom,
+    calc_sdom g = Some sdom ->
+    sdom (entry g) == L.top.
+
+  Axiom successors_sound : forall g sdom n1 n2,
+    calc_sdom g = Some sdom ->
+    Mem g n1 -> Mem g n2 -> Succ g n1 n2 -> 
+    L.union (L.singleton n1) (sdom n1) <= sdom n2.
+
+  Axiom complete : forall g sdom n1 n2,
+    calc_sdom g = Some sdom ->
+    SDom g n1 n2 -> L.In n1 (sdom n2).
+
+End Algdom.
+
+Module AlgdomProperties (Import G:GRAPH) (Import A : Algdom G).
+  Module Import GS := Spec G.
+
+  Lemma sound : forall g sdom n1 n2,
+    calc_sdom g = Some sdom ->              
+    L.In n1 (sdom n2) -> Dom g n1 n2.
+(* FOLD *)
+  Proof.
+    red; intros. remember (entry g). induction H1. subst.
+    pose proof entry_sound g sdom H. 
+
+    destruct (sdom (entry g)); try contradiction; simpl in *.
+      exfalso. rewrite H2 in H0. eapply L.SFacts.empty_iff. eauto.
+      
+    right. destruct (E.eq_dec v2 n1). subst. inversion H1; intuition.
+    apply IHPath; auto.
+
+    destruct (sdom v2) eqn:Heqv2; simpl in *; auto.
+    cut (NS.In n1 (NS.union (NS.singleton v2) t0)).
+    intro Hin. apply NS.union_1 in Hin as [Hin | Hin]; auto.
+    contradict n. apply NS.singleton_1. assumption.
+
+    pose proof successors_sound g sdom v2 v3 as Hss.
+    simpl in Hss. rewrite Heqv2 in Hss. simpl in Hss.
+    destruct (sdom v3). apply Hss; inversion H1; eauto.
+    exfalso. apply Hss; inversion H1; eauto.
+  Qed.
+(* /FOLD *)
+
+End AlgdomProperties.
+
